f_combined.v
@@ -1,0 +1,1021 @@
+From mm Require Import util abt abtutil.
+
+Module op.
+  Inductive t' :=
+  | arrow
+  | all
+  | bool
+
+  | abs
+  | app
+  | tyabs
+  | tyapp
+  | tt
+  | ff
+  | If
+  .
+  Definition t := t'.
+
+  Definition arity (op : t) : arity.t :=
+    match op with
+    | arrow => [0; 0]
+    | all => [1]
+    | bool => []
+
+    | abs => [0; 1]
+    | app => [0; 0]
+    | tyabs => [1]
+    | tyapp => [0; 0]
+    | tt => []
+    | ff => []
+    | If => [0; 0; 0]
+    end.
+
+  Definition eq_dec : forall x y : t, {x = y} + {x <> y}.
+    decide equality.
+  Defined.
+End op.
+
+Module abt := abt.abt op.
+
+Module ast.
+  Inductive t :=
+  | var (x : nat) : t
+  | arrow : t -> t -> t
+  | all : t -> t
+  | bool : t
+  | abs : t -> t -> t
+  | app : t -> t -> t
+  | tyabs : t -> t
+  | tyapp : t -> t -> t
+  | tt : t
+  | ff : t
+  | If : t -> t -> t -> t
+  .
+End ast.
+
+Module basis.
+  Module A := abt.
+
+  Import ast.
+  Definition t := t.
+
+  Fixpoint to_abt (term : t) : A.t :=
+    match term with
+    | var n => A.var n
+    | arrow ty1 ty2 => A.op op.arrow [A.bind 0 (to_abt ty1); A.bind 0 (to_abt ty2)]
+    | all ty => A.op op.all [A.bind 1 (to_abt ty)]
+    | bool => A.op op.bool []
+    | abs ty e => A.op op.abs [A.bind 0 (to_abt ty); A.bind 1 (to_abt e)]
+    | app e1 e2 => A.op op.app [A.bind 0 (to_abt e1); A.bind 0 (to_abt e2)]
+    | tyabs e => A.op op.tyabs [A.bind 1 (to_abt e)]
+    | tyapp e ty => A.op op.tyapp [A.bind 0 (to_abt e); A.bind 0 (to_abt ty)]
+    | tt => A.op op.tt []
+    | ff => A.op op.ff []
+    | If e1 e2 e3 => A.op op.If [A.bind 0 (to_abt e1);
+                               A.bind 0 (to_abt e2);
+                               A.bind 0 (to_abt e3)]
+    end.
+
+  Fixpoint of_abt (term : A.t) : t :=
+    match term with
+    | A.var n => var n
+    | A.op op.arrow [A.bind 0 a1; A.bind 0 a2] => arrow (of_abt a1) (of_abt a2)
+    | A.op op.all [A.bind 1 a'] => all (of_abt a')
+    | A.op op.bool [] => bool
+    | A.op op.abs [A.bind 0 a_ty; A.bind 1 a_e] => abs (of_abt a_ty) (of_abt a_e)
+    | A.op op.app [A.bind 0 a1; A.bind 0 a2] => app (of_abt a1) (of_abt a2)
+    | A.op op.tyabs [A.bind 1 a'] => tyabs (of_abt a')
+    | A.op op.tyapp [A.bind 0 a_e; A.bind 0 a_ty] => tyapp (of_abt a_e) (of_abt a_ty)
+    | A.op op.tt [] => tt
+    | A.op op.ff [] => ff
+    | A.op op.If [A.bind 0 a1; A.bind 0 a2; A.bind 0 a3] =>
+      If (of_abt a1) (of_abt a2) (of_abt a3)
+    | _ => var 0 (* bogus *)
+    end.
+
+  Fixpoint t_map ov c (term : t) : t :=
+    match term with
+    | var x => ov c x
+    | arrow ty1 ty2 => arrow (t_map ov c ty1) (t_map ov c ty2)
+    | all ty => all (t_map ov (S c) ty)
+    | bool => bool
+    | abs ty e => abs (t_map ov c ty) (t_map ov (S c) e)
+    | app e1 e2 => app (t_map ov c e1) (t_map ov c e2)
+    | tyabs e => tyabs (t_map ov (S c) e)
+    | tyapp e ty => tyapp (t_map ov c e) (t_map ov c ty)
+    | tt => tt
+    | ff => ff
+    | If e1 e2 e3 => If (t_map ov c e1) (t_map ov c e2) (t_map ov c e3)
+    end.
+
+  Fixpoint shift c d (term : t) : t :=
+    match term with
+    | var alpha => var (if alpha <? c then alpha else alpha + d)
+    | arrow ty1 ty2 => arrow (shift c d ty1) (shift c d ty2)
+    | all ty => all (shift (S c) d ty)
+    | bool => bool
+    | abs ty e => abs (shift c d ty) (shift (S c) d e)
+    | app e1 e2 => app (shift c d e1) (shift c d e2)
+    | tyabs e => tyabs (shift (S c) d e)
+    | tyapp e ty => tyapp (shift c d e) (shift c d ty)
+    | tt => tt
+    | ff => ff
+    | If e1 e2 e3 => If (shift c d e1) (shift c d e2) (shift c d e3)
+    end.
+
+  Fixpoint subst rho term :=
+    match term with
+    | var alpha => match nth_error rho alpha with
+                  | Some ty' => ty'
+                  | None => term
+                  end
+    | arrow ty1 ty2 => arrow (subst rho ty1) (subst rho ty2)
+    | all ty => all (subst (var 0 :: map (shift 0 1) rho) ty)
+    | bool => bool
+    | abs ty e => abs (subst rho ty) (subst (var 0 :: map (shift 0 1) rho) e)
+    | app e1 e2 => app (subst rho e1) (subst rho e2)
+    | tyabs e => tyabs (subst (var 0 :: map (shift 0 1) rho) e)
+    | tyapp e ty => tyapp (subst rho e) (subst rho ty)
+    | tt => tt
+    | ff => ff
+    | If e1 e2 e3 => If (subst rho e1) (subst rho e2) (subst rho e3)
+    end.
+
+  Fixpoint wf n term :=
+    match term with
+    | var alpha => alpha < n
+    | arrow ty1 ty2 => wf n ty1 /\ wf n ty2
+    | all ty => wf (S n) ty
+    | bool => True
+    | abs ty e => wf n ty /\ wf (S n) e
+    | app e1 e2 => wf n e1 /\ wf n e2
+    | tyabs e => wf (S n) e
+    | tyapp e ty => wf n e /\ wf n ty
+    | tt => True
+    | ff => True
+    | If e1 e2 e3 => wf n e1 /\ wf n e2 /\ wf n e3
+    end.
+
+  Fixpoint identity_subst (n : nat) : list t :=
+    match n with
+    | 0 => []
+    | S n => var 0 :: map (shift 0 1) (identity_subst n)
+    end.
+
+  Lemma ws_to_abt : forall e, A.ws (to_abt e).
+  Proof. A.basis_util.prove_ws_to_abt. Qed.
+
+  Lemma of_to_abt : forall e, of_abt (to_abt e) = e.
+  Proof. A.basis_util.prove_of_to_abt. Qed.
+
+  Lemma to_of_abt : forall a, A.ws a -> to_abt (of_abt a) = a.
+  Proof. A.basis_util.prove_to_of_abt to_abt of_abt. Qed.
+
+  Lemma t_map_to_abt_comm : forall ov e c,
+      to_abt (t_map ov c e) = A.t_map (fun c x => to_abt (ov c x)) c (to_abt e).
+  Proof. A.basis_util.prove_t_map_to_abt_comm. Qed.
+
+  Lemma shift_to_abt_comm : forall e c d, to_abt (shift c d e) = A.shift c d (to_abt e).
+  Proof. A.basis_util.prove_shift_to_abt_comm. Qed.
+
+  Lemma map_shift_to_abt_comm :
+    forall c d rho, map to_abt (map (shift c d) rho) = map (A.shift c d) (map to_abt rho).
+  Proof. A.basis_util.prove_map_shift_to_abt_comm shift_to_abt_comm. Qed.
+
+  Lemma subst_to_abt_comm : forall e rho,
+      to_abt (subst rho e) = A.subst (map to_abt rho) (to_abt e).
+  Proof. A.basis_util.prove_subst_to_abt_comm t map_shift_to_abt_comm. Qed.
+
+  Lemma wf_to_abt : forall e n, wf n e <-> A.wf n (to_abt e).
+  Proof. A.basis_util.prove_wf_to_abt. Qed.
+
+  Lemma identity_subst_to_abt_comm :
+    forall n, List.map to_abt (identity_subst n) = A.identity_subst n.
+  Proof. A.basis_util.prove_identity_subst_to_abt_comm map_shift_to_abt_comm. Qed.
+
+  Definition var := var.
+  Arguments var /.
+  Lemma var_to_abt : forall n, to_abt (var n) = A.var n.
+  Proof. reflexivity. Qed.
+End basis.
+
+Module term.
+  Include abt_util basis.
+  Notation arrow := ast.arrow.
+  Notation all := ast.all.
+  Notation bool := ast.bool.
+  Notation abs := ast.abs.
+  Notation app := ast.app.
+  Notation tyabs := ast.tyabs.
+  Notation tyapp := ast.tyapp.
+  Notation tt := ast.tt.
+  Notation ff := ast.ff.
+  Notation If := ast.If.
+End term.
+
+Module cat.
+  Inductive t := TYPE | EXPR.
+End cat.
+
+Module wc.
+  Inductive t : list cat.t -> term.t -> cat.t -> Prop :=
+  | var : forall C n c,
+      nth_error C n = Some c ->
+      t C (term.var n) c
+  | arrow : forall C t1 t2,
+      t C t1 cat.TYPE ->
+      t C t2 cat.TYPE ->
+      t C (term.arrow t1 t2) cat.TYPE
+  | all : forall C ty,
+      t (cat.TYPE :: C) ty cat.TYPE ->
+      t C (term.all ty) cat.TYPE
+  | bool : forall C,
+      t C ast.bool cat.TYPE
+  | abs : forall C ty e,
+      t C ty cat.TYPE ->
+      t (cat.EXPR :: C) e cat.EXPR ->
+      t C (term.abs ty e) cat.EXPR
+  | app : forall C e1 e2,
+      t C e1 cat.EXPR ->
+      t C e2 cat.EXPR ->
+      t C (term.app e1 e2) cat.EXPR
+  | tyabs : forall C e,
+      t (cat.TYPE :: C) e cat.EXPR ->
+      t C (term.tyabs e) cat.EXPR
+  | tyapp : forall C e ty,
+      t C e cat.EXPR ->
+      t C ty cat.TYPE ->
+      t C (term.tyapp e ty) cat.EXPR
+  | tt : forall C,
+      t C term.tt cat.EXPR
+  | ff : forall C,
+      t C term.ff cat.EXPR
+  | If : forall C e1 e2 e3,
+      t C e1 cat.EXPR ->
+      t C e2 cat.EXPR ->
+      t C e3 cat.EXPR ->
+      t C (term.If e1 e2 e3) cat.EXPR
+  .
+  Hint Constructors t : core.
+
+  Lemma t_wf :
+    forall C e c,
+      t C e c ->
+      term.wf (length C) e.
+  Proof.
+    induction 1; cbn; intuition.
+    apply nth_error_Some.
+    congruence.
+  Qed.
+
+  Lemma shift :
+    forall C1 C2 C3 e c,
+      t (C1 ++ C3) e c ->
+      t (C1 ++ C2 ++ C3) (term.shift (length C1) (length C2) e) c.
+  Proof.
+    intros C1 C2 C3 e c WC.
+    revert C2.
+    remember (C1 ++ C3) as C eqn:EC in *.
+    revert C1 C3 EC.
+    induction WC; intros C1 C3 EC C2; subst C; cbn [term.shift]; constructor; auto.
+    - now rewrite nth_error_shift.
+    - now apply IHWC with (C2 := _ :: _).
+    - now apply IHWC2 with (C2 := _ :: _).
+    - now apply IHWC with (C2 := _ :: _).
+  Qed.
+
+  Lemma shift' :
+    forall C e c C',
+      t C e c ->
+      t (C' ++ C) (term.shift 0 (List.length C') e) c.
+  Proof.
+    intros.
+    now apply shift with (C1 := []).
+  Qed.
+
+  Lemma shift_cons :
+  forall C e c c',
+    t C e c ->
+    t (c' :: C) (term.shift 0 1 e) c.
+  Proof.
+    intros C e c c' HT.
+    now apply shift' with (C' := [c']).
+  Qed.
+
+  Lemma t_skipn_shift :
+    forall C e c n,
+      n <= length C ->
+      t (skipn n C) e c ->
+      t C (term.shift 0 n e) c.
+  Proof.
+    intros C e c n L T.
+    rewrite <- firstn_skipn with (n := n) (l := C).
+    apply shift' with (C' := firstn n C) in T.
+    now rewrite firstn_length_le in * by assumption.
+  Qed.
+
+  Lemma shift_inv :
+  forall e C1 C2 C3 c,
+    t (C1 ++ C2 ++ C3) (term.shift (length C1) (length C2) e) c ->
+    t (C1 ++ C3) e c.
+  Proof.
+    induction e; intros C1 C2 C3 c HT; invc HT; constructor; eauto.
+    - now rewrite nth_error_shift in *.
+    - eapply IHe with (C1 := _ :: _); eauto.
+    - eapply IHe2 with (C1 := _ :: _); eauto.
+    - eapply IHe with (C1 := _ :: _); eauto.
+  Qed.
+
+  Lemma shift_inv' :
+    forall C e c C',
+      t (C' ++ C) (term.shift 0 (List.length C') e) c ->
+      t C e c.
+  Proof.
+    intros.
+    now eapply shift_inv with (C1 := []); eauto.
+  Qed.
+
+  Lemma shift_cons_inv :
+  forall C e c c',
+    t (c' :: C) (term.shift 0 1 e) c ->
+    t C e c.
+  Proof.
+    intros C e c c' HT.
+    now apply shift_inv' with (C' := [c']).
+  Qed.
+
+  Lemma subst :
+    forall C e c,
+      t C e c ->
+      forall C' rho,
+        List.Forall2 (t C') rho C ->
+        t C' (term.subst rho e) c.
+  Proof.
+    induction 1; intros C' rho F; cbn [term.subst]; try constructor;
+      eauto 10 using shift_cons, Forall2_impl, Forall2_map_l.
+    cbn.
+    destruct (Forall2_nth_error2 F H) as [z [Hz Ht]].
+    unfold term.t in Hz.
+    now rewrite Hz.
+  Qed.
+
+  Lemma Forall2_identity_subst :
+    forall C n,
+      n = length C ->
+      Forall2 (t C) (term.identity_subst n) C.
+  Proof.
+    intros C n ?. subst n.
+    induction C; cbn; constructor.
+    - auto.
+    - apply Forall2_map_l.
+      eauto using Forall2_impl, shift_cons.
+  Qed.
+
+  Lemma Forall2_t_Forall_wf :
+    forall C es tys,
+      Forall2 (wc.t C) es tys ->
+      Forall (term.wf (length C)) es.
+  Proof.
+    induction 1; eauto using t_wf.
+  Qed.
+End wc.
+
+Module ctx_ent.
+  Inductive t :=
+  | TYVAR
+  | EXVAR : term.t -> t
+  .
+
+  Definition map (f : term.t -> term.t) (ce : t) : t :=
+    match ce with
+    | TYVAR => TYVAR
+    | EXVAR t => EXVAR (f t)
+    end.
+
+  Definition prop (P : term.t -> Prop) (ce : t) : Prop :=
+    match ce with
+    | TYVAR => True
+    | EXVAR t => P t
+    end.
+
+  Definition to_cat (ce : t) : cat.t :=
+    match ce with
+    | TYVAR => cat.TYPE
+    | EXVAR _ => cat.EXPR
+    end.
+
+  Module exports.
+    Notation TYVAR := TYVAR.
+    Notation EXVAR := EXVAR.
+  End exports.
+End ctx_ent.
+
+Module tele.
+  Import ctx_ent.exports.
+
+  Definition t := list ctx_ent.t.
+
+  Notation to_cat_ctx T := (map ctx_ent.to_cat T).
+  Notation map f := (map (ctx_ent.map f)).
+
+  Fixpoint wf (T : t) : Prop :=
+    match T with
+    | [] => True
+    | ce :: T =>
+      wf T /\ ctx_ent.prop (fun ty => wc.t (to_cat_ctx T) ty cat.TYPE) ce
+    end.
+
+  Fixpoint shift (c d : nat) (T : t) : t :=
+    match T with
+    | [] => []
+    | ce :: T =>
+      match c with
+      | 0 => ctx_ent.map (term.shift c d) ce :: shift c d T
+      | S c => ctx_ent.map (term.shift c d) ce :: shift c d T
+      end
+    end.
+
+  Lemma shift_length :
+    forall T c d,
+      length (shift c d T) = length T.
+  Proof.
+    induction T; intros [|] d; cbn; auto.
+  Qed.
+
+  Definition is_tyvar (T : t) (n : nat) : Prop :=
+    nth_error T n = Some TYVAR.
+
+  Definition lookup_exvar (T : t) (n : nat) (expect : term.t) : Prop :=
+    exists expect',
+      nth_error T n = Some (EXVAR expect') /\
+      expect = term.shift 0 (S n) expect'.
+
+  Fixpoint globalize (i : nat) (T : t) : list ctx_ent.t :=
+    match T with
+    | [] => []
+    | ce :: T =>
+      ctx_ent.map (term.shift 0 (S i)) ce :: globalize (S i) T
+    end.
+
+  Lemma nth_error_globalize :
+    forall T i n,
+      nth_error (globalize i T) n =
+      match nth_error T n with
+      | None => None
+      | Some e => Some (ctx_ent.map (term.shift 0 (n + S i)) e)
+      end.
+  Proof.
+    induction T; intros i [|n]; cbn; auto.
+    rewrite IHT.
+    break_match; auto.
+    repeat f_equal.
+    lia.
+  Qed.
+
+  Lemma lookup_exvar_globalize :
+    forall T n ty,
+      lookup_exvar T n ty ->
+      nth_error (globalize 0 T) n = Some (EXVAR ty).
+  Proof.
+    intros T n ty [ty' [NE ?]].
+    subst ty.
+    rewrite nth_error_globalize, NE.
+    cbn.
+    repeat f_equal.
+    lia.
+  Qed.
+
+  Lemma to_cat_shift :
+    forall T c d,
+      to_cat_ctx (shift c d T) = to_cat_ctx T.
+  Proof.
+    unfold ctx_ent.to_cat.
+    induction T; cbn [List.map shift]; intros c d.
+    - reflexivity.
+    - destruct c, a; cbn; f_equal; auto.
+  Qed.
+
+  Lemma nth_error_tele_shift_exvar1 :
+    forall T c d n ty,
+      nth_error (shift c d T) n = Some (EXVAR ty) ->
+      exists ty',
+        term.shift (c - S n) d ty' = ty /\
+        nth_error T n = Some (EXVAR ty').
+  Proof.
+    induction T; intros [|c] d [|n] ty NE; cbn in *; try discriminate.
+    - unfold ctx_ent.map in *. destruct a; try congruence.
+      invc NE. eauto.
+    - apply IHT in NE. assumption.
+    - destruct a; cbn in *; try congruence.
+      invc NE.
+      rewrite Nat.sub_0_r.
+      eauto.
+    - auto.
+  Qed.
+
+  Lemma nth_error_tele_shift_exvar2 :
+    forall T c d n ty,
+      nth_error T n = Some (EXVAR ty) ->
+      nth_error (shift c d T) n = Some (EXVAR (term.shift (c - S n) d ty)).
+  Proof.
+    induction T; intros [|c] d [|n] ty NE; cbn in *; try discriminate.
+    - invc NE; reflexivity.
+    - now erewrite IHT by eassumption.
+    - rewrite Nat.sub_0_r.
+      invc NE; reflexivity.
+    - eauto.
+  Qed.
+
+  Lemma lookup_exvar_shift :
+    forall T1 T2 T3 n expect,
+     lookup_exvar (shift (length T1) (length T2) T1 ++ T2 ++ T3)
+                  (if n <? length T1 then n else n + length T2)
+                  (term.shift (length T1) (length T2) expect) <->
+     lookup_exvar (T1 ++ T3) n expect.
+  Proof.
+    intros T1 T2 T3 n expect.
+    unfold lookup_exvar.
+    rewrite nth_error_shift' in * by now rewrite shift_length.
+    destruct (Nat.ltb_spec n (length T1)).
+    - rewrite !nth_error_app1 by now rewrite ?shift_length.
+      split; intros [expect' [NE ?]]; subst.
+      + apply nth_error_tele_shift_exvar1 in NE.
+        destruct NE as [ty' [Ety' NE]].
+        subst. eexists. split; [eassumption|].
+        rewrite term.shift_shift in * by lia.
+        replace (length T1 - S n + S n) with (length T1) in * by lia.
+        eauto using term.shift_inj.
+      + erewrite nth_error_tele_shift_exvar2 by eassumption.
+        eexists. split; [reflexivity|].
+        rewrite term.shift_shift with (c2 := 0) by lia.
+        f_equal. lia.
+    - rewrite !nth_error_app2 by (rewrite ?shift_length; lia).
+      rewrite shift_length.
+      split; intros [expect' [NE ?]]; subst;
+        (eexists; split; [eassumption|]).
+      + apply term.shift_inj with (c := length T1) (d := length T2).
+        now rewrite term.shift_merge by lia.
+      + now rewrite term.shift_merge by lia.
+  Qed.
+
+  Lemma lookup_exvar_nth_error :
+    forall T n ty,
+      lookup_exvar T n ty ->
+      exists ty',
+        nth_error T n = Some (EXVAR ty').
+  Proof.
+    intros T n ty LE.
+    unfold lookup_exvar in *.
+    destruct LE as [expect' [NE ?]]. subst.
+    eauto.
+  Qed.
+
+  Lemma nth_error_wc :
+    forall T n ty,
+      nth_error T n = Some (EXVAR ty) ->
+      wf T ->
+      wc.t (skipn (S n) (to_cat_ctx T)) ty cat.TYPE.
+  Proof.
+    induction T; cbn; intros n ty NE WF; destruct n; try discriminate.
+    - invc NE. intuition.
+    - apply IHT; intuition.
+  Qed.
+
+  Lemma lookup_exvar_wc :
+    forall T n ty,
+      lookup_exvar T n ty ->
+      wf T ->
+      wc.t (to_cat_ctx T) ty cat.TYPE.
+  Proof.
+    intros T n ty [expect' [NE ?]] WFT. subst.
+    apply wc.t_skipn_shift.
+    - apply lt_le_S. apply nth_error_Some.
+      rewrite nth_error_map, NE.
+      discriminate.
+    - auto using nth_error_wc.
+  Qed.
+
+  Lemma to_cat_ctx_cons :
+    forall ce T,
+      to_cat_ctx (cons ce T) = ctx_ent.to_cat ce :: to_cat_ctx T.
+  Proof. reflexivity. Qed.
+
+  Lemma wf_cons_exvar :
+    forall ty T,
+      wc.t (to_cat_ctx T) ty cat.TYPE ->
+      wf T ->
+      wf (cons (EXVAR ty) T).
+  Proof. cbn. auto. Qed.
+
+  Lemma wf_cons_tyvar :
+    forall T,
+      wf T ->
+      wf (cons TYVAR T).
+  Proof. cbn. auto. Qed.
+
+  Lemma to_cat_ctx_globalize :
+    forall (G : t) i,
+      to_cat_ctx (globalize i G) =
+      to_cat_ctx G.
+  Proof.
+    induction G; cbn; intros i.
+    - reflexivity.
+    - f_equal; [|now auto].
+      destruct a; reflexivity.
+  Qed.
+
+  Lemma to_cat_ctx_subst :
+    forall rho G,
+      to_cat_ctx (List.map (ctx_ent.map (term.subst rho)) G) =
+      to_cat_ctx G.
+  Proof.
+    induction G; cbn.
+    - reflexivity.
+    - f_equal; [|now auto].
+      destruct a; reflexivity.
+  Qed.
+
+  Lemma globalize_length :
+    forall G i,
+      length (tele.globalize i G) = length G.
+  Proof.
+    induction G; cbn; intros i; auto.
+  Qed.
+
+  Lemma globalize_0 :
+    forall G i,
+      globalize i G = List.map (ctx_ent.map (term.shift 0 i)) (globalize 0 G).
+  Proof.
+    induction G; intros i; cbn; f_equal.
+    - destruct a; cbn; f_equal; auto.
+      now rewrite term.shift_merge by lia.
+    - rewrite IHG with (i := S i).
+      rewrite IHG with (i := 1).
+      rewrite map_map.
+      apply map_ext.
+      clear.
+      intros [|ty]; cbn; f_equal; auto.
+      now rewrite term.shift_merge by lia.
+  Qed.
+
+  Lemma wf_globalize :
+    forall G,
+      tele.wf G ->
+      Forall (ctx_ent.prop (term.wf (length G))) (tele.globalize 0 G).
+  Proof.
+    intros G WF.
+    induction G; cbn in *; constructor; destruct WF as [WF HA].
+    - destruct a as [|ty]; cbn in *; auto.
+      apply wc.t_wf in HA.
+      apply term.wf_shift'.
+      now rewrite map_length in HA.
+    - forward IHG.
+      rewrite globalize_0.
+      rewrite Forall_map.
+      eapply Forall_impl; [|eassumption].
+      clear.
+      intros [|ty]; cbn; intros WF; auto using term.wf_shift'.
+  Qed.
+End tele.
+
+Module has_type.
+  Import ctx_ent.exports.
+
+  Inductive t : tele.t -> term.t -> term.t -> Prop :=
+  | var : forall G x ty,
+      tele.lookup_exvar G x ty ->
+      t G (term.var x) ty
+  | abs : forall G ty1 ty2 ty2' e,
+      wc.t (tele.to_cat_ctx G) ty1 cat.TYPE ->
+      t (EXVAR ty1 :: G) e ty2 ->
+      ty2 = term.shift 0 1 ty2' ->
+      t G (term.abs ty1 e) (term.arrow ty1 ty2')
+  | app : forall G ty1 ty2 e1 e2,
+      t G e1 (term.arrow ty1 ty2) ->
+      t G e2 ty1 ->
+      t G (term.app e1 e2) ty2
+  | tyabs : forall G e ty,
+      t (TYVAR :: G) e ty ->
+      t G (term.tyabs e) (term.all ty)
+  | tyapp : forall G e ty_body ty,
+      wc.t (tele.to_cat_ctx G) ty cat.TYPE ->
+      t G e (term.all ty_body) ->
+      t G (term.tyapp e ty) (term.subst (ty :: term.identity_subst (length G)) ty_body)
+  | tt : forall G,
+      t G term.tt term.bool
+  | ff : forall G,
+      t G term.ff term.bool
+  | If : forall G e1 e2 e3 ty,
+      t G e1 term.bool ->
+      t G e2 ty ->
+      t G e3 ty ->
+      t G (term.If e1 e2 e3) ty
+  .
+  Hint Constructors t : core.
+
+  Lemma t_wc_e :
+    forall G e ty,
+      t G e ty ->
+      tele.wf G ->
+      wc.t (tele.to_cat_ctx G) e cat.EXPR.
+  Proof.
+    induction 1; cbn in *; intros TWF; auto.
+    constructor.
+    destruct (tele.lookup_exvar_nth_error _ _ _ H) as [ty' NE].
+    now erewrite map_nth_error by eassumption.
+  Qed.
+
+  Lemma t_wc_ty :
+    forall G e ty,
+      t G e ty ->
+      tele.wf G ->
+      wc.t (map ctx_ent.to_cat G) ty cat.TYPE.
+  Proof.
+    induction 1; cbn in *; intros TWF; auto.
+    - destruct (tele.lookup_exvar_nth_error _ _ _ H) as [ty' NE].
+      eauto using tele.lookup_exvar_wc.
+    - constructor; auto.
+      forward IHt.
+      subst ty2.
+      eauto using wc.shift_cons_inv.
+    - forward IHt1.
+      now invc IHt1.
+    - forward IHt.
+      invc IHt.
+      eapply wc.subst; eauto.
+      constructor; [assumption|].
+      apply wc.Forall2_identity_subst.
+      now rewrite map_length.
+  Qed.
+
+  Lemma shift :
+  forall G1 G2 G3 e ty,
+    tele.wf (G1 ++ G3) ->
+    has_type.t (G1 ++ G3) e ty ->
+    has_type.t (tele.shift (length G1) (length G2) G1 ++ G2 ++ G3)
+               (term.shift (length G1) (length G2) e)
+               (term.shift (length G1) (length G2) ty).
+  Proof.
+    intros G1 G2 G3 e ty WF HT.
+    revert G2.
+    remember (G1 ++ G3) as G eqn:EG in *.
+    revert WF G1 G3 EG.
+    induction HT; intros WF G1 G3 EG G2; subst G; cbn [term.shift]; eauto.
+    - constructor.
+      now rewrite tele.lookup_exvar_shift.
+    - econstructor; [| |reflexivity].
+      + rewrite !map_app in *.
+        apply wc.shift with (C2 := map ctx_ent.to_cat G2) in H.
+        eqapply H.
+        * now rewrite !map_length.
+        * now rewrite tele.to_cat_shift.
+      + rewrite term.shift_shift with (c2 := 0) by lia.
+        forward IHHT.
+        specialize (IHHT (_ :: _) _ eq_refl G2).
+        subst ty2.
+        eqapply IHHT.
+        f_equal. cbn. lia.
+    - econstructor.
+      forward IHHT.
+      eapply (IHHT (_ :: _) _ eq_refl).
+    - specialize (IHHT ltac:(auto) _ _ eq_refl G2).
+      assert (term.wf (length (ty :: term.identity_subst (length (G1 ++ G3)))) ty_body).
+      {
+        cbn. rewrite term.identity_subst_length.
+        apply t_wc_ty in HT; [|assumption].
+        apply wc.t_wf in HT.
+        rewrite map_length in HT.
+        apply HT.
+      }
+      rewrite term.shift_subst by assumption.
+      cbn [term.shift] in IHHT.
+      eapply tyapp in IHHT.
+      eqapply IHHT.
+      + rewrite !app_length, tele.shift_length.
+        rewrite term.identity_subst_app.
+        rewrite term.SIS_app.
+        rewrite app_comm_cons.
+        rewrite term.subst_shift.
+        * cbn. f_equal. f_equal.
+          rewrite term.identity_subst_app, map_app.
+          rewrite term.map_shift_identity_subst'.
+          f_equal.
+          rewrite term.SIS_merge by lia.
+          f_equal.
+          lia.
+        * rewrite ?app_length, ?term.SIS_length in *.
+          cbn in *.
+          now rewrite term.identity_subst_length in *.
+        * cbn.
+          now rewrite term.identity_subst_length in *.
+        * now rewrite term.SIS_length.
+      + rewrite !map_app in *.
+        rewrite tele.to_cat_shift.
+        eapply wc.shift in H.
+        eqapply H.
+        now rewrite !map_length.
+  Qed.
+
+  Lemma shift' :
+    forall G e ty G',
+      tele.wf G ->
+      t G e ty ->
+      t (G' ++ G) (term.shift 0 (List.length G') e) (term.shift 0 (List.length G') ty).
+  Proof.
+    intros.
+    now apply shift with (G1 := []).
+  Qed.
+
+  Lemma shift_cons :
+  forall G e ty ty',
+    tele.wf G ->
+    has_type.t G e ty ->
+    has_type.t (ty' :: G) (term.shift 0 1 e) (term.shift 0 1 ty).
+  Proof.
+    intros G e ty ty' WF HT.
+    now apply shift' with (G' := [ty']).
+  Qed.
+
+  Definition t_ctx_ent G e ce :=
+    match ce with
+    | TYVAR => wc.t (tele.to_cat_ctx G) e cat.TYPE
+    | EXVAR ty => t G e ty
+    end.
+
+  Lemma Forall2_t_ctx_ent_wc :
+    forall G es tys,
+      tele.wf G ->
+      Forall2 (t_ctx_ent G) es tys ->
+      Forall2 (wc.t (tele.to_cat_ctx G)) es (map ctx_ent.to_cat tys).
+  Proof.
+    intros G es tys WF F.
+    apply Forall2_map_r.
+    eapply Forall2_impl; [|eassumption].
+    intros.
+    destruct b; cbn in *.
+    - assumption.
+    - eapply t_wc_e; eauto.
+  Qed.
+
+  Lemma subst :
+    forall G e ty,
+      t G e ty ->
+      tele.wf G ->
+      forall G' rho,
+        tele.wf G' ->
+        List.Forall2 (t_ctx_ent G') rho
+                     (map (ctx_ent.map (term.subst rho)) (tele.globalize 0 G)) ->
+        t G' (term.subst rho e) (term.subst rho ty).
+  Proof.
+    induction 1; intros WFG G' rho WFG' F; cbn [term.subst]; eauto;
+      assert (length G = length rho) as L
+        by (apply Forall2_length in F;
+            rewrite map_length, tele.globalize_length in F;
+            congruence).
+    - pose proof (tele.lookup_exvar_globalize _ _ _ ltac:(eassumption)).
+      pose proof (map_nth_error (ctx_ent.map (term.subst rho)) _ _ H0).
+      destruct (Forall2_nth_error2 F ltac:(eassumption)) as [z [Hz Ht]].
+      cbn.
+      unfold term.t in *. (* ugh *)
+      now rewrite Hz.
+    - apply abs with (ty2 := term.subst (term.descend 1 rho) ty2).
+      + eapply wc.subst.
+        eassumption.
+        apply Forall2_t_ctx_ent_wc in F; [|assumption].
+        eqapply F.
+        now rewrite tele.to_cat_ctx_subst, tele.to_cat_ctx_globalize.
+      + forward IHt.
+        apply IHt.
+        {
+          cbn; split; [assumption|].
+          eapply wc.subst; [eassumption|].
+          apply Forall2_t_ctx_ent_wc in F; [|assumption].
+          now rewrite tele.to_cat_ctx_subst, tele.to_cat_ctx_globalize in F.
+        }
+        {
+          cbn.
+          constructor.
+          - unfold t_ctx_ent.
+            constructor.
+            eexists.
+            cbn.
+            split;[reflexivity|].
+            assert (term.wf (length rho) ty1).
+            {
+              apply wc.t_wf in H.
+              rewrite map_length in H.
+              congruence.
+            }
+            rewrite term.shift_subst by assumption.
+            now rewrite term.subst_shift_cons by now rewrite map_length.
+          - assert (Forall2
+                      (t_ctx_ent (EXVAR (term.subst rho ty1) :: G'))
+                      (List.map (term.shift 0 1) rho)
+                      (List.map
+                         (ctx_ent.map (term.shift 0 1))
+                         (List.map (ctx_ent.map (term.subst rho)) (tele.globalize 0 G))))
+              as F'.
+            {
+              (* basically apply shift_cons in F. *)
+              rewrite map_map.
+              rewrite Forall2_map.
+              rewrite Forall2_map_r_iff in F.
+              eapply Forall2_impl; [|eassumption].
+              cbn.
+              (* this should be a lemma *)
+              intros a [|ty]; cbn; intros Hty.
+              - auto using wc.shift_cons.
+              - auto using shift_cons.
+            }
+
+            eqapply F'.
+            rewrite tele.globalize_0 with (i := 1).
+            rewrite !map_map.
+            apply tele.wf_globalize in WFG.
+            apply map_ext_Forall.
+            eapply Forall_impl; [|eassumption].
+            clear -L.
+            intros [|ty] WF; cbn in *; [reflexivity|f_equal].
+            rewrite term.shift_subst by congruence.
+            now rewrite term.subst_shift_cons by (rewrite map_length; congruence).
+        }
+      + subst ty2.
+        apply term.subst_descend_shift_shift_subst.
+        apply t_wc_ty in H0.
+        apply wc.t_wf in H0.
+        rewrite map_length in *.
+        cbn [length] in H0.
+        apply term.wf_shift_inv' in H0.
+        congruence.
+        cbn. split; auto.
+    - econstructor.
+      apply IHt; cbn; auto.
+      constructor; [now cbn; auto|].
+      rewrite Forall2_map_r_iff in F.
+      rewrite tele.globalize_0.
+      rewrite map_map.
+      apply Forall2_map.
+      eapply Forall_Forall2_and_r in F; [|apply tele.wf_globalize; assumption].
+      eapply Forall2_impl; [|eassumption].
+      cbn.
+      intros a [|tyb] [HT WF]; cbn in *.
+      + auto using wc.shift_cons.
+      + rewrite term.subst_cons_shift_shift_subst_1 by congruence.
+        now apply shift_cons; auto.
+    - forward IHt.
+      specialize (IHt G' rho ltac:(assumption) ltac:(assumption)).
+      cbn in IHt.
+      apply tyapp with (ty := term.subst rho ty) in IHt.
+      2: {
+        eapply wc.subst; eauto.
+        apply Forall2_t_ctx_ent_wc in F; [|assumption].
+        eqapply F.
+        now rewrite tele.to_cat_ctx_subst, tele.to_cat_ctx_globalize.
+      }
+      eqapply IHt.
+      rewrite !term.subst_subst.
+      + f_equal. cbn. f_equal.
+        rewrite map_map.
+        rewrite L.
+        rewrite term.map_subst_identity_subst.
+        erewrite map_ext_Forall; [now apply map_id|].
+        apply Forall2_t_ctx_ent_wc in F; [|assumption].
+        apply wc.Forall2_t_Forall_wf in F.
+        rewrite map_length in F.
+        eapply Forall_impl; [|eassumption].
+        intros a WF.
+        rewrite term.subst_shift_cons by now rewrite term.identity_subst_length.
+        now rewrite term.subst_identity.
+      + cbn. rewrite term.identity_subst_length.
+        (* this should be a lemma *)
+        apply t_wc_ty in H0; [|assumption].
+        apply wc.t_wf in H0.
+        rewrite map_length in H0.
+        apply H0.
+      + constructor; auto.
+        apply wc.t_wf in H.
+        rewrite map_length in H.
+        congruence.
+        rewrite L.
+        apply term.wf_identity_subst.
+      + cbn.
+        apply t_wc_ty in H0; [|assumption].
+        apply wc.t_wf in H0.
+        rewrite !map_length in *.
+        rewrite L in H0.
+        apply H0.
+      + constructor; auto.
+        * cbn. lia.
+        * apply Forall_map.
+          apply Forall2_t_ctx_ent_wc in F; [|assumption].
+          apply wc.Forall2_t_Forall_wf in F.
+          eapply Forall_impl; [|eassumption].
+          intros a.
+          cbn.
+          rewrite map_length.
+          rewrite term.identity_subst_length.
+          auto using term.wf_shift'.
+  Qed.
+End has_type.
+Print Assumptions has_type.subst.
